code/hash/Hacl.Hash.Blake2.fst
@@ -1,0 +1,16 @@
+module Hacl.Hash.Blake2
+
+let update_multi_blake2s: update_multi_st Blake2S =
+  admit()
+let update_multi_blake2b: update_multi_st Blake2B =
+  admit()
+
+let update_last_blake2s: update_last_st Blake2S =
+  admit()
+let update_last_blake2b: update_last_st Blake2B =
+  admit()
+
+let hash_blake2s: hash_st Blake2S =
+  admit()
+let hash_blake2b: hash_st Blake2B =
+  admit()
