code/hash/Hacl.Hash.Blake2.fsti
@@ -1,0 +1,15 @@
+module Hacl.Hash.Blake2
+
+open Spec.Hash.Definitions
+open Hacl.Hash.Definitions
+
+include Hacl.Hash.Core.Blake2
+
+val update_multi_blake2s: update_multi_st Blake2S
+val update_multi_blake2b: update_multi_st Blake2B
+
+val update_last_blake2s: update_last_st Blake2S
+val update_last_blake2b: update_last_st Blake2B
+
+val hash_blake2s: hash_st Blake2S
+val hash_blake2b: hash_st Blake2B
